WIP on more instances

theories/Torch/Tensor/Instances.v
@@ -1,1095 +1,305 @@
 From Coq.Structures Require Import Equalities.
 From Coq Require Import ZArith Sint63 Uint63 List PArray Lia Setoid Morphisms.
 From NeuralNetInterp.Util Require Nat.
-From NeuralNetInterp.Util Require Import Wf_Uint63 PArray.Proofs PArray.Instances List.Proofs Default Pointed PArray List Notations Arith.Classes Arith.Instances Bool (*PrimitiveProd*).
+From NeuralNetInterp.Util Require Import Wf_Uint63 Wf_Uint63.Instances PArray.Proofs PArray.Instances List.Proofs Default Pointed PArray List Notations Arith.Classes Arith.Instances Bool (*PrimitiveProd*).
 From NeuralNetInterp.Torch Require Import Tensor.
 
-Definition eqf {r A s} : relation (@tensor r A s)
-  := (eq ==> eq)%signature.
+Definition eqfR {r A s} R : relation (@tensor r A s)
+  := pointwise_relation _ R.
+Notation eqf := (eqfR eq).
 
-#[export] Instance eqf_Reflexive {r A s} : Reflexive (@eqf r A s).
+#[export] Instance eqf_Reflexive {r A s R} {_ : Reflexive R} : Reflexive (@eqfR r A s R).
 Proof. repeat intro; subst; reflexivity. Qed.
-#[export] Instance eqf_Symmetric {r A s} : Symmetric (@eqf r A s).
+#[export] Instance eqf_Symmetric {r A s R} {_ : Symmetric R} : Symmetric (@eqfR r A s R).
 Proof. cbv; repeat intro; subst; symmetry; auto. Qed.
-#[export] Instance eqf_Transitive {r A s} : Transitive (@eqf r A s).
-Proof. intros x y z H1 H2 i i' ?; subst; etransitivity; [ eapply H1 | eapply H2 ]; reflexivity. Qed.
-
-
-
-Import Util.Nat.Notations.
-Import Util.Wf_Uint63.LoopNotation.
-Import Util.Wf_Uint63.Reduction.
-Import Arith.Classes.
-Local Open Scope list_scope.
-Set Implicit Arguments.
-Import ListNotations.
-(*Import PrimitiveProd.Primitive.*)
-
-Definition Rank := nat.
-#[global] Bind Scope nat_scope with Rank.
-#[local] Coercion is_true : bool >-> Sortclass.
-
-Module Type IndexType.
-  Parameter t : Type.
-  Notation IndexType := t.
-End IndexType.
-
-Module Type ExtendedIndexType.
-  Include IndexType.
-  Parameter zero : has_zero t.
-  Parameter one : has_one t.
-  Parameter leb : has_leb t.
-  Parameter ltb : has_ltb t.
-  Parameter eqb : has_eqb t.
-  Parameter mul : has_mul t.
-  Parameter add : has_add t.
-  Parameter int_div : has_int_div t.
-  Parameter modulo : has_mod t.
-  #[export] Existing Instances eqb one zero ltb leb mul add int_div modulo.
-End ExtendedIndexType.
-
-Module IndexGen.
-  Module Make (IndexType : IndexType).
-    Import (hints) IndexType.
-    Notation IndexType := IndexType.t.
-
-    Fixpoint t (r : Rank) : Type
-      := match r with
-         | O => unit
-         | S r => t r * IndexType.t
-         end.
-    Notation Index := t.
-
-    Definition nil : t 0 := tt.
-    Definition snoc {r} (s : t r) x : t (S r) := (s, x).
-    Module Import IndexNotations0.
-      Declare Scope index_scope.
-      Delimit Scope index_scope with index.
-      Bind Scope index_scope with Index.
-      Notation "xs ::' x" := (snoc xs x) : index_scope.
-      Notation "[ ]" := nil : index_scope.
-      Notation "[ x ]" := (snoc nil x) : index_scope.
-      Notation "[ x ; y ; .. ; z ]" :=  (snoc .. (snoc (snoc nil x) y) .. z) : index_scope.
-    End IndexNotations0.
-    Module IndexPatternNotations.
-      Declare Scope index_pattern_scope.
-      Delimit Scope index_pattern_scope with index_pattern.
-      Notation "xs ::' x" := (pair xs x) : index_pattern_scope.
-      Notation "[ ]" := tt : index_pattern_scope.
-      Notation "[ x ]" := (pair tt x) : index_pattern_scope.
-      Notation "[ x ; y ; .. ; z ]" :=  (pair .. (pair (pair tt x) y) .. z) : index_pattern_scope.
-    End IndexPatternNotations.
-    #[local] Open Scope index_scope.
-    Definition hd {r : Rank} : Index (S r) -> Index r := @fst _ _.
-    Definition tl {r : Rank} : Index (S r) -> IndexType := @snd _ _.
-    Fixpoint app {r1 r2 : Rank} {struct r2} : Index r1 -> Index r2 -> Index (r1 +' r2)
-      := match r2 with
-         | 0%nat => fun sz _tt => sz
-         | S r2 => fun sz1 sz2 => @app r1 r2 sz1 (hd sz2) ::' tl sz2
-         end%index.
-    Definition cons {r : Rank} x (xs : Index r) : Index _ := app [x] xs.
-    Module Export IndexNotations1.
-      Include IndexNotations0.
-      Notation "x :: xs" := (cons x xs) : index_scope.
-      Notation "s1 ++ s2" := (app s1 s2) : index_scope.
-      Notation "s1 ++' s2" := (app s1 s2) : index_scope.
-    End IndexNotations1.
-
-    Section repeat.
-      Context (x : IndexType).
-      Fixpoint repeat (r : Rank) : Index r
-        := match r with
-           | O => []
-           | S r => repeat r ::' x
-           end.
-
-      Lemma hd_repeat {r} : hd (repeat (S r)) = repeat r.
-      Proof using Type. reflexivity. Qed.
-
-      Lemma tl_repeat {r} : tl (repeat (S r)) = x.
-      Proof using Type. reflexivity. Qed.
-    End repeat.
-
-    Definition item : Index 1 -> IndexType := tl.
-
-    Fixpoint map {r} (f : IndexType -> IndexType) : Index r -> Index r
-      := match r with
-         | 0%nat => fun _ => []
-         | S r => fun xs => map f (hd xs) ::' f (tl xs)
-         end.
-
-    Fixpoint map2 {r} (f : IndexType -> IndexType -> IndexType) : Index r -> Index r -> Index r
-      := match r with
-         | 0%nat => fun _ _ => []
-         | S r => fun xs ys => map2 f (hd xs) (hd ys) ::' f (tl xs) (tl ys)
-         end.
-
-    (* TODO: nary *)
-    Fixpoint map3 {r} (f : IndexType -> IndexType -> IndexType -> IndexType) : Index r -> Index r -> Index r -> Index r
-      := match r with
-         | 0%nat => fun _ _ _ => []
-         | S r => fun xs ys zs => map3 f (hd xs) (hd ys) (hd zs) ::' f (tl xs) (tl ys) (tl zs)
-         end.
-
-    Fixpoint fold_map {A B r} (f : IndexType -> A) (accum : B -> A -> B) (init : B) : Index r -> B
-      := match r with
-         | 0%nat => fun _ => init
-         | S r => fun xs => fold_map f accum (accum init (f (tl xs))) (hd xs)
-         end.
-
-    Fixpoint fold_map2 {A B r} (f : IndexType -> IndexType -> A) (accum : B -> A -> B) (init : B) : Index r -> Index r -> B
-      := match r with
-         | 0%nat => fun _ _ => init
-         | S r => fun xs ys => fold_map2 f accum (accum init (f (tl xs) (tl ys))) (hd xs) (hd ys)
-         end.
-
-    Fixpoint curriedT_dep {r : Rank} : (Index r -> Type) -> Type
-      := match r with
-         | O => fun f => f []
-         | S r => fun f => curriedT_dep (fun init => forall i, f (init ::' i))
-         end.
-    Definition curriedT {r} (T : Type) : Type := @curriedT_dep r (fun _ => T).
-
-    Fixpoint curry_dep {r} : forall {T}, (forall i : Index r, T i) -> @curriedT_dep r T
-      := match r return forall {T}, (forall i : Index r, T i) -> @curriedT_dep r T with
-         | O => fun T f => f []
-         | S r => fun T f => @curry_dep r _ (fun rest i => f (rest ::' i))
-         end.
-    Definition curry {r T} : (Index r -> T) -> @curriedT r T
-      := @curry_dep r (fun _ => T).
-    Fixpoint uncurry_map_dep {r} : forall {A B}, (forall i, A i -> B i) -> @curriedT_dep r A -> (forall i : Index r, B i)
-      := match r return forall {A B}, (forall i, A i -> B i) -> @curriedT_dep r A -> (forall i : Index r, B i) with
-         | O => fun A B F f 'tt => F _ f
-         | S r => fun A B F f '(rest, i)
-                  => @uncurry_map_dep
-                       r (fun rest => forall i, A (rest ::' i)) (fun rest => B (rest ::' i))
-                       (fun rest f => F _ (f _))
-                       f rest
-         end.
-    Definition uncurry_dep {r} {T} : @curriedT_dep r T -> (forall i : Index r, T i)
-      := @uncurry_map_dep r T T (fun _ x => x).
-    Definition uncurry {r T} : @curriedT r T -> (Index r -> T)
-      := uncurry_dep.
-
-    Fixpoint split_radd {r1 r2} {struct r2} : Index (r1 +' r2) -> Index r1 * Index r2
-      := match r2 with
-         | 0%nat => fun idx => (idx, tt)
-         | S r2
-           => fun '(idx1, idx2)
-              => let '(idx11, idx12) := @split_radd r1 r2 idx1 in
-                 (idx11, (idx12, idx2))
-         end.
-    Fixpoint combine_radd {r1 r2} {struct r2} : Index r1 * Index r2 -> Index (r1 +' r2)
-      := match r2 return Index r1 * Index r2 -> Index (r1 +' r2) with
-         | 0%nat => fun '(idx, tt) => idx
-         | S r2
-           => fun '(idx1, (idx2, idx3))
-              => (@combine_radd r1 r2 (idx1, idx2), idx3)
-         end.
-
-    Definition curry_radd {A r1 r2} : (Index (r1 +' r2) -> A) -> (Index r1 -> Index r2 -> A)
-      := fun f i1 i2 => f (combine_radd (i1, i2)).
-    Definition uncurry_radd {A r1 r2} : (Index r1 -> Index r2 -> A) -> (Index (r1 +' r2) -> A)
-      := fun f i => let '(i1, i2) := split_radd i in f i1 i2.
-    Definition curry_S {A r} : (Index (1 +' r) -> A) -> (Index 1 -> Index r -> A)
-      := curry_radd.
-    Definition uncurry_S {A r} : (Index 1 -> Index r -> A) -> (Index (1 +' r) -> A)
-      := uncurry_radd.
-
-    Module UncurryNotation.
-      Notation "'uncurry_fun' x1 .. xn => body"
-        := (match _ return _ with
-            | ty => uncurry_S (fun x1 => .. (uncurry_S (fun xn => match body return Index 0 -> ty with v => fun 'tt => v end)) .. )
-            end)
-             (only parsing, at level 200, x1 binder, xn binder, body at level 200).
-    End UncurryNotation.
-
-    Module Export IndexNotations.
-      Include IndexNotations1.
-      (*Include UncurryNotation.*)
-    End IndexNotations.
-
-    Module UncurryCoercions.
-      Coercion uncurry_dep : curriedT_dep >-> Funclass.
-      Coercion uncurry : curriedT >-> Funclass.
-    End UncurryCoercions.
-
-    Fixpoint droplastn {r : Rank} (n : Rank) : Index r -> Index (r -' n)
-      := match n, r with
-         | 0%nat, _ => fun xs => xs
-         | _, 0%nat => fun _tt => []
-         | S n, S r => fun xs => @droplastn r n (hd xs)
-         end.
-
-    Fixpoint lastn {r : Rank} (n : Rank) : Index r -> Index (Nat.min n r)
-      := match n, r return Index r -> Index (Nat.min n r) with
-         | 0%nat, _ => fun _ => []
-         | _, 0%nat => fun _ => []
-         | S n, S r => fun xs => lastn n (hd xs) ::' (tl xs)
-         end.
-
-    Fixpoint reduce {A} (reduction : A -> IndexType -> A) (init : A) {r} : Index r -> A
-      := match r with
-         | 0%nat => fun _ => init
-         | S r => fun idxs => reduction (reduce reduction init (hd idxs)) (tl idxs)
-         end.
-  End Make.
-
-  Module Type MakeSig (IndexType : IndexType) := Nop <+ Make IndexType.
-
-  Module ExtendedMake (IndexType : ExtendedIndexType).
-    Import (hints) IndexType.
-    Include Make IndexType.
-    Import IndexNotations.
-    #[local] Open Scope index_scope.
-
-    Definition ones {r} := repeat 1%core r.
-
-    #[export] Instance eqb {r : Rank} : has_eqb (Index r)
-      := fold_map2 IndexType.eqb andb true.
-    #[export] Instance leb {r : Rank} : has_leb (Index r)
-      := fold_map2 IndexType.leb andb true.
-    #[export] Instance ltb {r : Rank} : has_ltb (Index r)
-      := match r with O => fun _ _ => false | _ => fold_map2 IndexType.ltb andb true end.
-    Lemma expand_eqb {r} (xs ys : Index (S r)) : ((xs =? ys) = ((hd xs =? hd ys) && (@Classes.eqb _ IndexType.eqb (tl xs) (tl ys))))%core%bool.
-    Proof.
-      cbv [Classes.eqb]; cbn.
-      set (b := IndexType.eqb _ _); clearbody b.
-      revert b; induction r as [|r IH]; cbn; try reflexivity; intros.
-      rewrite !IH; destruct b, IndexType.eqb, eqb; reflexivity.
-    Qed.
-    Lemma expand_leb {r} (xs ys : Index (S r)) : ((xs <=? ys) = ((hd xs <=? hd ys) && (tl xs <=? tl ys)))%core%bool.
-    Proof.
-      cbv [Classes.leb]; cbn.
-      set (b := IndexType.leb _ _); clearbody b.
-      revert b; induction r as [|r IH]; cbn; try reflexivity; intros.
-      rewrite !IH; destruct b, IndexType.leb, leb; reflexivity.
-    Qed.
-    Lemma expand_ltb {r} (xs ys : Index (S r)) : ((xs <? ys) = (match r with O => true | _ => hd xs <? hd ys end && (@Classes.ltb _ IndexType.ltb (tl xs) (tl ys))))%core%bool.
-    Proof.
-      cbv [Classes.ltb ltb]; cbn.
-      set (b := IndexType.ltb _ _); clearbody b.
-      revert b; induction r as [|r IH]; cbn; try reflexivity; intros.
-      rewrite !IH; destruct b, IndexType.ltb, r; try reflexivity.
-      all: destruct fold_map2; reflexivity.
-    Qed.
-
-    Module Rank.
-      Fixpoint filter {r : Rank} (f : IndexType -> bool) : Index r -> Rank
-        := match r with
-           | 0%nat => fun _ => 0%nat
-           | S r => fun idx => @filter r f (hd idx) +' if f (tl idx) then 1 else 0
-           end.
-      Definition squeeze {r : Rank} (i : Index r) : Rank
-        := filter (fun i => (i != 1)%core) i.
-    End Rank.
-    Fixpoint filter {r : Rank} (f : IndexType -> bool) : forall i : Index r, Index (Rank.filter f i)
-      := match r return forall i : Index r, Index (Rank.filter f i) with
-         | 0%nat => fun _ => []
-         | S r => fun idx => @filter r f (hd idx) ++' if f (tl idx) as ftlidx return Index (if ftlidx then _ else _) then [tl idx] else []
-         end.
-
-    Definition squeeze {r : Rank} (i : Index r) : Index (Rank.squeeze i)
-      := filter (fun i => (i != 1)%core) i.
-
-    Fixpoint unfilter {r : Rank} (f : IndexType -> bool) : forall {i : Index r}, Index (Rank.filter f i) -> Index r
-      := match r return forall i : Index r, Index (Rank.filter f i) -> Index r with
-         | 0%nat => fun _ idxs => idxs
-         | S r
-           => fun idx
-              => if f (tl idx) as ftlidx return Index (_ +' if ftlidx then 1 else 0) -> Index (S r)
-                 then fun idxs => @unfilter r f (hd idx) (hd idxs) ::' tl idxs
-                 else fun idxs => @unfilter r f (hd idx) idxs ::' 0
-         end%core.
-
-    Definition unsqueeze {r : Rank} {i : Index r} : Index (Rank.squeeze i) -> Index r
-      := unfilter (fun i => (i != 1)%core).
-
-    Definition prod {r} : Index r -> IndexType
-      := reduce mul 1%core.
-  End ExtendedMake.
-
-  Module Type ExtendedMakeSig (IndexType : ExtendedIndexType) := Nop <+ ExtendedMake IndexType.
-End IndexGen.
-
-Module Shape.
-  Module ShapeType <: ExtendedIndexType.
-    Definition t : Type := int.
-    #[global] Strategy 100 [t].
-    #[global] Bind Scope uint63_scope with t.
-    Definition one : has_one t := _.
-    Definition zero : has_zero t := _.
-    Definition eqb : has_eqb t := _.
-    Definition mul : has_mul t := _.
-    Definition add : has_add t := _.
-    Definition int_div : has_int_div t := _.
-    Definition modulo : has_mod t := _.
-    (* eta expand to get around COQBUG(https://github.com/coq/coq/issues/17663) *)
-    Definition leb : has_leb t := fun x y => Uint63.leb x y.
-    Definition ltb : has_ltb t := fun x y => Uint63.ltb x y.
-  End ShapeType.
-
-  Include IndexGen.ExtendedMake ShapeType.
-
-  Module Export ShapeNotations.
-    Declare Scope shape_scope.
-    Delimit Scope shape_scope with shape.
-    Bind Scope shape_scope with t.
-    Bind Scope uint63_scope with IndexType.
-    Notation "xs ::' x" := (snoc xs x) : shape_scope.
-    Notation "[ ]" := nil : shape_scope.
-    Notation "[ x ]" := (snoc nil x) : shape_scope.
-    Notation "[ x ; y ; .. ; z ]" :=  (snoc .. (snoc (snoc nil x) y) .. z) : shape_scope.
-    Notation "x :: xs" := (cons x xs) : shape_scope.
-    Notation "s1 ++ s2" := (app s1 s2) : shape_scope.
-    Notation "s1 ++' s2" := (app s1 s2) : shape_scope.
-  End ShapeNotations.
-
-  Definition broadcast2 {r} : Index r -> Index r -> Index r
-    := map2 max.
-  Definition broadcast3 {r} : Index r -> Index r -> Index r -> Index r
-    := map3 (fun a b c => max (max a b) c).
-
-  Definition reshape' {r} : Index r -> Z
-    := Shape.reduce (fun z x => z * Uint63.to_Z x)%Z 1%Z.
-  Definition reshape {r} (s : Index r) : Index 1
-    := [Uint63.of_Z (reshape' s)].
-End Shape.
-Notation ShapeType := Shape.IndexType.
-Notation Shape := Shape.Index.
-Export Shape.ShapeNotations.
-Export (hints) Shape.
-
-Module RawIndex.
-  Module RawIndexType <: ExtendedIndexType.
-    Definition t : Type := int.
-    #[global] Strategy 100 [t].
-    #[global] Bind Scope uint63_scope with t.
-    Definition one : has_one t := _.
-    Definition zero : has_zero t := _.
-    Definition eqb : has_eqb t := _.
-    Definition mul : has_mul t := _.
-    Definition add : has_add t := _.
-    Definition int_div : has_int_div t := _.
-    Definition modulo : has_mod t := _.
-    (* eta expand to get around COQBUG(https://github.com/coq/coq/issues/17663) *)
-    Definition leb : has_leb t := fun x y => Uint63.leb x y.
-    Definition ltb : has_ltb t := fun x y => Uint63.ltb x y.
-  End RawIndexType.
-
-  Include IndexGen.ExtendedMake RawIndexType.
-
-  Module Export RawIndexNotations.
-    Declare Scope raw_index_scope.
-    Delimit Scope raw_index_scope with raw_index.
-    Bind Scope raw_index_scope with t.
-    Bind Scope uint63_scope with IndexType.
-    Notation "xs ::' x" := (snoc xs x) : raw_index_scope.
-    Notation "[ ]" := nil : raw_index_scope.
-    Notation "[ x ]" := (snoc nil x) : raw_index_scope.
-    Notation "[ x ; y ; .. ; z ]" :=  (snoc .. (snoc (snoc nil x) y) .. z) : raw_index_scope.
-    Notation "x :: xs" := (cons x xs) : raw_index_scope.
-    Notation "s1 ++ s2" := (app s1 s2) : raw_index_scope.
-    Notation "s1 ++' s2" := (app s1 s2) : raw_index_scope.
-  End RawIndexNotations.
-
-  Fixpoint reshape' {r} : Shape r -> Index r -> Z
-    := match r with
-       | 0%nat => fun s idx => 0
-       | S r
-         => fun s idx
-            => Uint63.to_Z (tl idx) + @reshape' r (Shape.hd s) (hd idx) * Uint63.to_Z (Shape.tl s)
-       end%Z%core%raw_index.
-
-  Fixpoint unreshape' {r} : Shape r -> Z -> Index r
-    := match r with
-       | 0%nat => fun _ _ => []
-       | S r
-         => fun s idx
-            => let tl_idx := idx mod (Uint63.to_Z (Shape.tl s)) in
-               let hd_idx := idx // (Uint63.to_Z (Shape.tl s)) in
-               @unreshape' r (Shape.hd s) hd_idx ::' Uint63.of_Z tl_idx
-       end%Z%core%raw_index.
-
-  Definition reshape {r} (s : Shape r) (idx : Index r) : Index 1 := [Uint63.of_Z (reshape' s idx)].
-  Definition unreshape {r} (s : Shape r) (idx : Index 1) : Index r := unreshape' s (Uint63.to_Z (item idx)).
-
-  Lemma unrereshape' {r} s idx : (match r with 0%nat => true | _ => idx <? s end)%core -> @unreshape' r s (@reshape' r s idx) = idx /\ (0 <= @reshape' r s idx < Shape.reshape' s)%Z.
-  Proof.
-    induction r; [ | rewrite expand_ltb ];
-      cbv [Shape.reshape'] in *;
-      cbn [Shape Index unreshape' reshape' Shape.reduce] in *;
-      cbv [is_true Shape.hd Shape.tl snoc nil hd tl fst snd Classes.int_div Classes.add Classes.mul Classes.modulo Z_has_int_div] in *;
-      repeat match goal with H : unit |- _ => destruct H | H : _ * _ |- _ => destruct H end; try (split; try reflexivity; lia);
-      cbv [Classes.ltb RawIndexType.ltb Uint63.ltb] in *.
-    all: rewrite Bool.andb_true_iff, Z_mod_plus_full, Uint63.ltb_spec.
-    all: intros [H0 H1].
-    repeat match goal with
-           | [ |- context[to_Z ?x] ]
-             => let lem := constr:(to_Z_bounded x) in
-                let ty := type of lem in
-                lazymatch goal with
-                | [ _ : ty |- _ ] => fail
-                | _ => idtac
-                end;
-                pose proof lem
-           end.
-    rewrite Z.mod_small, Z_div_plus_full, Z.div_small, Z.add_0_l, Uint63.of_to_Z by lia.
-    destruct r;
-      [ cbn [Shape Index unreshape' reshape' Shape.reduce] in *;
-        cbv [is_true Shape.hd Shape.tl snoc nil hd tl fst snd Classes.int_div Classes.add Classes.mul Classes.modulo Z_has_int_div] in *;
-        repeat match goal with H : unit |- _ => destruct H | H : _ * _ |- _ => destruct H end; split; try reflexivity; lia
-      | ].
-    specialize (IHr _ _ ltac:(eassumption)).
-    destruct IHr as [IHr1 IHr2].
-    rewrite IHr1; split; try reflexivity.
-    nia.
-  Qed.
-
-  Lemma reunreshape' {r} s idx : (0 <= idx < Shape.reshape' s)%Z -> @reshape' r s (@unreshape' r s idx) = idx /\ (match r with 0%nat => true | _ => @unreshape' r s idx <? s end)%core.
-  Proof.
-    revert idx; induction r; intro idx; [ | rewrite expand_ltb ];
-      cbv [Shape.reshape'] in *;
-      cbn [Shape Index unreshape' reshape' Shape.reduce] in *;
-      cbv [is_true Shape.hd Shape.tl snoc nil hd tl fst snd Classes.int_div Classes.add Classes.mul Classes.modulo Z_has_int_div] in *;
-      repeat match goal with H : unit |- _ => destruct H | H : _ * _ |- _ => destruct H end; try (split; try reflexivity; lia);
-      cbv [Classes.ltb RawIndexType.ltb Uint63.ltb] in *.
-    all: rewrite Bool.andb_true_iff, Uint63.ltb_spec, !Uint63.of_Z_spec.
-    intro H.
-    repeat match goal with
-           | [ |- context[to_Z ?x] ]
-             => let lem := constr:(to_Z_bounded x) in
-                let ty := type of lem in
-                lazymatch goal with
-                | [ _ : ty |- _ ] => fail
-                | _ => idtac
-                end;
-                pose proof lem
-           | [ |- context[(?x mod ?y)%Z] ]
-             => let lem := constr:(Z.mod_pos_bound x y ltac:(lia)) in
-                let ty := type of lem in
-                lazymatch goal with
-                | [ _ : ty |- _ ] => fail
-                | _ => idtac
-                end;
-                pose proof lem
-           | [ H : (0 <= ?idx < ?x * ?y)%Z |- _ ]
-             => lazymatch goal with
-                | [ _ : (0 < y)%Z |- _ ] => fail
-                | _ => idtac
-                end;
-                assert (0 < x)%Z by nia;
-                assert (0 < y)%Z by nia
-           end.
-    rewrite ?Z.mod_small by lia.
-    match goal with
-    | [ |- context[reshape' ?s (unreshape' ?s ?idx)] ]
-      => specialize (IHr s idx)
-    end.
-    specialize (IHr ltac:(Z.to_euclidean_division_equations; nia)).
-    destruct IHr as [IHr1 IHr2].
-    rewrite IHr1; repeat split; try (now destruct r); try lia; [].
-    Z.to_euclidean_division_equations; nia.
-  Qed.
-End RawIndex.
-Notation RawIndexType := RawIndex.IndexType.
-Notation RawIndex := RawIndex.Index.
-Export RawIndex.RawIndexNotations.
-Export (hints) RawIndex.
-
-Module Index.
-  Module IndexType <: ExtendedIndexType.
-    Definition t : Type := int.
-    #[global] Strategy 100 [t].
-    #[global] Bind Scope sint63_scope with t.
-    Definition one : has_one t := _.
-    Definition zero : has_zero t := _.
-    Definition eqb : has_eqb t := _.
-    Definition mul : has_mul t := _.
-    Definition add : has_add t := _.
-    Definition int_div : has_int_div t := _.
-    Definition modulo : has_mod t := _.
-    (* eta expand to get around COQBUG(https://github.com/coq/coq/issues/17663) *)
-    Definition leb : has_leb t := fun x y => Sint63.leb x y.
-    Definition ltb : has_ltb t := fun x y => Sint63.ltb x y.
-  End IndexType.
-
-  Include IndexGen.ExtendedMake IndexType.
-  Export IndexNotations.
-  Bind Scope sint63_scope with IndexType.
-End Index.
-Notation IndexType := Index.IndexType.
-Notation Index := Index.Index.
-Export Index.IndexNotations.
-Export (hints) Index.
-Bind Scope sint63_scope with Index.IndexType.
-
-(*
-Definition tensor_of_rank@{a r} (A : Type@{a}) (r : Rank)
-  := RawIndex@{r} r -> A.
-(* we could have a separate universe for the shape, but since the shape argument is a phantom one anyway, we don't bother *)
-Definition tensor@{a r} {r : Rank} (A : Type@{a}) (s : Shape@{r} r)
-  := tensor_of_rank@{a r} A r.
-*)
-Monomorphic Definition tensor_of_rank (A : Type) (r : Rank) : Type
-  := RawIndex r -> A.
-Monomorphic Definition tensor {r : Rank} (A : Type) (s : Shape r) : Type
-  := tensor_of_rank A r.
-
-Monomorphic Definition tensor_dep {r A s} (P : A -> Type) (x : @tensor r A s)
-  := forall i : RawIndex r, P (x i).
-
-Definition tensor_undep {r A s P x} (t : @tensor_dep r A s (fun _ => P) x) : @tensor r P s
-  := t.
-
-Declare Scope tensor_scope.
-Delimit Scope tensor_scope with tensor.
-Declare Scope raw_tensor_scope.
-Delimit Scope raw_tensor_scope with raw_tensor.
-Bind Scope tensor_scope with tensor_of_rank.
-Bind Scope tensor_scope with tensor.
-Local Open Scope tensor_scope.
-
-Definition eqf {r A s} : relation (@tensor r A s)
-  := (eq ==> eq)%signature.
-
-#[export] Instance eqf_Reflexive {r A s} : Reflexive (@eqf r A s).
-Proof. repeat intro; subst; reflexivity. Qed.
-#[export] Instance eqf_Symmetric {r A s} : Symmetric (@eqf r A s).
-Proof. cbv; repeat intro; subst; symmetry; auto. Qed.
-#[export] Instance eqf_Transitive {r A s} : Transitive (@eqf r A s).
-Proof. intros x y z H1 H2 i i' ?; subst; etransitivity; [ eapply H1 | eapply H2 ]; reflexivity. Qed.
-
-#[export] Instance empty_of_rank {A r} {default : pointed A} : pointed (tensor_of_rank A r)
-  := fun _ => default.
-#[export] Instance empty {r A} {default : pointed A} {s : Shape r} : pointed (tensor A s)
-  := empty_of_rank.
-
-#[export] Typeclasses Opaque Index.
-
-Ltac get_shape val :=
-  lazymatch type of val with
-  | tensor _ ?shape => shape
-  | list ?x
-    => let len := (eval cbv in (Uint63.of_Z (Z.of_N (N.of_nat (List.length val))))) in
-       let rest := lazymatch (eval hnf in val) with
-                   | cons ?val _ => get_shape val
-                   | ?val => fail 1 "Could not find cons in" val
-                   end in
-       constr:(Shape.cons len rest)
-  | array ?x
-    => let len := (eval cbv in (PArray.length val)) in
-       let rest := let val := (eval cbv in (PArray.get val 0)) in
-                   get_shape val in
-       constr:(Shape.cons len rest)
-  | _ => constr:(Shape.nil)
-  end.
-Notation shape_of x := (match x return _ with y => ltac:(let s := get_shape y in exact s) end) (only parsing).
-Class compute_shape_of {A r} (x : A) := get_shape_of : Shape r.
-#[global] Hint Extern 0 (compute_shape_of ?x) => let s := get_shape x in exact s : typeclass_instances.
+#[export] Instance eqf_Transitive {r A s R} {_ : Transitive R} : Transitive (@eqfR r A s R).
+Proof. intros x y z H1 H2; repeat intro; subst; etransitivity; [ eapply H1 | eapply H2 ]; reflexivity. Qed.
 
 Module PArray.
-  Fixpoint concrete_tensor_of_rank (A : Type) (r : Rank) : Type
-    := match r with
-       | O => A
-       | S r => concrete_tensor_of_rank (array A) r
-       end.
-  Definition concrete_tensor {r : Rank} (A : Type) (s : Shape r) : Type
-    := concrete_tensor_of_rank A r.
-  #[global] Strategy 100 [tensor_of_rank tensor concrete_tensor concrete_tensor_of_rank].
-
-  Module Tensor.
-    Fixpoint map {r A B} (f : A -> B) : forall {s}, @concrete_tensor r A s -> @concrete_tensor r B s
-      := match r return forall {s}, @concrete_tensor r A s -> @concrete_tensor r B s with
-         | O => fun _ => f
-         | S r => fun s t => @map r _ _ (PArray.map f) (Shape.hd s) t
-         end.
-    Definition copy {r A s} t := @map r A A (fun x => x) s t.
-  End Tensor.
-
-  Fixpoint concretize {r : Rank} {A : Type} {default : pointed A} {struct r} : forall {s : Shape r} (t : tensor A s), concrete_tensor A s
-    := match r with
-       | 0%nat => fun _tt f => f tt
-       | S r
-         => fun '(s, len) f
-            => concretize (r:=r) (A:=array A) (s:=s) (fun idxs => PArray.init_default len (fun idx => f (idxs, idx)))
-       end.
-  Fixpoint abstract_of_rank {r : Rank} {A : Type} {struct r}
-    : concrete_tensor_of_rank A r -> tensor_of_rank A r
-    := match r with
-       | O => fun v _tt => v
-       | S r => fun t '(idxs, idx) => PArray.get (@abstract_of_rank r (array A) t idxs) idx
-       end.
-  Definition abstract {r : Rank} {A : Type} {s : Shape r} : concrete_tensor A s -> tensor A s
-    := abstract_of_rank.
-
-  Notation to_tensor t := (@abstract _ _ (shape_of t%array) t%array) (only parsing).
-
+  Import Tensor.PArray.
   #[export] Instance concretize_Proper {r A default s} : Proper (eqf ==> eq) (@concretize r A default s).
   Proof.
     cbv [eqf Proper respectful]; revert A default s; induction r; cbn [concretize]; intros A default s t1 t2 H; auto; [].
     destruct s.
-    eapply IHr.
-    Locate init_default.
-    destr
-    { apply H. }
-Proof. intros x y z H1 H2 i i' ?; subst; etransitivity; [ eapply H1 | eapply H2 ]; reflexivity. Qed.
-
-
-  Lemma abstract_concretize {r A default} {s : Shape r} {t} {idxs : RawIndex r}
-    (in_bounds : is_true (match r with O => true | _ => idxs <? s end)%core)
-    (in_max_bounds : is_true (match r with O => true | _ => idxs <? RawIndex.repeat PArray.max_length r end)%core)
-    : abstract (@concretize r A default s t) idxs = t idxs.
-  Proof.
-    cbv [abstract].
-    revert A default idxs t in_bounds in_max_bounds; induction r as [|r IH]; cbn [abstract_of_rank concretize]; intros.
-    { destruct idxs; reflexivity. }
-    { cbv [is_true] in *.
-      rewrite RawIndex.expand_ltb, Bool.andb_true_iff in in_bounds, in_max_bounds.
-      destruct idxs, s.
-      rewrite IH by first [ apply in_bounds | apply in_max_bounds ].
-      rewrite PArray.get_init_default.
-      rewrite RawIndex.tl_repeat in *.
-      cbv [Classes.ltb Classes.leb RawIndex.RawIndexType.ltb RawIndex.tl] in *.
-      cbn [RawIndex.hd RawIndex.tl RawIndex.repeat] in *.
-      cbn in *.
-      do 2 destruct PrimInt63.ltb; destruct in_bounds, in_max_bounds; try congruence; cbn.
-      reflexivity. }
+    eapply IHr; repeat intro; subst.
+    apply PArray.init_default_Proper; try reflexivity; repeat intro; subst.
+    apply H.
   Qed.
 
-  Definition reabstract {r : Rank} {A s} (t_ : @tensor r A s) (t : @concrete_tensor r A s) : @tensor r A s
-    := let t := abstract t in
-       fun idxs
-       => if ((idxs <? s) && (idxs <? RawIndex.repeat PArray.max_length r))%core%bool
-          then t idxs
-          else t_ idxs.
+  #[export] Instance reabstract_Proper {r A s} : Proper (eqf ==> eq ==> eqf) (@reabstract r A s).
+  Proof. cbv [reabstract]; repeat intro; subst; destruct andb; eauto. Qed.
 
-  Lemma reabstract_correct {r A} {s : Shape r} {t_} {t} {idxs : RawIndex r}
-    : (forall
-          (in_bounds : is_true (match r with O => true | _ => idxs <? s end)%core)
-          (in_max_bounds : is_true (match r with O => true | _ => idxs <? RawIndex.repeat PArray.max_length r end)%core),
-          abstract t idxs = t_ idxs)
-      -> @reabstract r A s t_ t idxs = t_ idxs.
-  Proof.
-    cbv [reabstract].
-    cbv [andb].
-    repeat match goal with |- context[match ?x with _ => _ end] => destruct x eqn:? end.
-    all: repeat match goal with H : context[match ?x with _ => _ end] |- _ => destruct x eqn:? end.
-    all: auto.
-    all: discriminate.
-  Qed.
-
-  Lemma reabstract_ext_correct {r A default} {s : Shape r} {t_ t}
-    : t = @concretize r A default s t_ -> forall idxs, @reabstract r A s t_ t idxs = t_ idxs.
-  Proof. intros; subst; apply reabstract_correct, abstract_concretize. Qed.
-
-  Definition checkpoint {r : Rank} {A default s} t : @tensor r A s
-    := let t_ := t in
-       let t := @concretize r A default s t in
-       reabstract t_ t.
-
-  Lemma checkpoint_correct {r A default} {s : Shape r} {t} {idxs : RawIndex r}
-    : @checkpoint r A default s t idxs = t idxs.
-  Proof. cbv [checkpoint]; apply reabstract_ext_correct; reflexivity. Qed.
+  #[export] Instance checkpoint_Proper {r A default s} : Proper (eqf ==> eqf) (@checkpoint r A default s).
+  Proof. cbv [checkpoint]; repeat intro; subst; apply reabstract_Proper; try apply concretize_Proper; auto. Qed.
 End PArray.
+Export (hints) PArray.
 
 Module List.
-  Fixpoint concrete_tensor_of_rank (A : Type) (r : Rank) : Type
-    := match r with
-       | O => A
-       | S r => concrete_tensor_of_rank (list A) r
-       end.
-  Definition concrete_tensor {r : Rank} (A : Type) (s : Shape r) : Type
-    := concrete_tensor_of_rank A r.
-  #[global] Strategy 100 [tensor_of_rank tensor concrete_tensor concrete_tensor_of_rank].
-
-  Module Tensor.
-    Fixpoint map {r A B} (f : A -> B) : forall {s}, @concrete_tensor r A s -> @concrete_tensor r B s
-      := match r return forall {s}, @concrete_tensor r A s -> @concrete_tensor r B s with
-         | O => fun _ => f
-         | S r => fun s t => @map r _ _ (List.map f) (Shape.hd s) t
-         end.
-    Definition copy {r A s} t := @map r A A (fun x => x) s t.
-  End Tensor.
-
-  Fixpoint concretize {r : Rank} {A : Type} {struct r} : forall {s : Shape r} (t : tensor A s), concrete_tensor A s
-    := match r return forall {s : Shape r} (t : tensor A s), concrete_tensor A s with
-       | 0%nat => fun _tt f => f tt
-       | S r
-         => fun '(s, len) f
-            => concretize (r:=r) (A:=list A) (s:=s) (fun idxs => List.map (fun idx => f (idxs, Uint63.of_Z (Z.of_nat idx))) (List.seq 0 (Z.to_nat (Uint63.to_Z len))))
-       end.
-  Fixpoint abstract_of_rank {r : Rank} {A : Type} {default : pointed A} {struct r}
-    : concrete_tensor_of_rank A r -> tensor_of_rank A r
-    := match r return concrete_tensor_of_rank A r -> tensor_of_rank A r with
-       | O => fun v _tt => v
-       | S r => fun t '(idxs, idx) => nth_default default (@abstract_of_rank r (list A) _ t idxs) (Z.to_nat (Uint63.to_Z idx))
-       end.
-  Definition abstract {r : Rank} {A : Type} {default : pointed A} {s : Shape r} : concrete_tensor A s -> tensor A s
-    := abstract_of_rank.
-
-  Notation to_tensor t := (@abstract _ _ _ (shape_of t%list) t%list) (only parsing).
-
-  Lemma abstract_concretize {r A} {default : pointed A} {s : Shape r} {t} {idxs : RawIndex r}
-    (in_bounds : is_true (match r with O => true | _ => idxs <? s end)%core)
-    : abstract (@concretize r A s t) idxs = t idxs.
+  Import Tensor.List.
+  #[export] Instance concretize_Proper {r A s} : Proper (eqf ==> eq) (@concretize r A s).
   Proof.
-    cbv [abstract].
-    revert A default idxs t in_bounds; induction r as [|r IH]; cbn [abstract_of_rank concretize]; intros.
-    { destruct idxs; reflexivity. }
-    { cbv [is_true] in *.
-      rewrite RawIndex.expand_ltb, Bool.andb_true_iff in in_bounds.
-      destruct idxs as [idxs idx], s as [ss s].
-      rewrite IH by first [ apply in_bounds | apply in_max_bounds ].
-      cbv [nth_default].
-      rewrite nth_error_map.
-      rewrite List.nth_error_seq.
-      cbv [Classes.ltb Classes.leb RawIndex.RawIndexType.ltb RawIndex.tl] in *.
-      cbn in in_bounds.
-      rewrite Uint63.ltb_spec in in_bounds.
-      destruct (Uint63.to_Z_bounded idx).
-      destruct (Uint63.to_Z_bounded s).
-      destruct Nat.ltb eqn:H'; cbn [option_map].
-      1:rewrite Nat.ltb_lt, <- Z2Nat.inj_lt in H' by assumption.
-      2:rewrite Nat.ltb_ge, <- Z2Nat.inj_le in H' by assumption.
-      1: rewrite Nat.add_0_l, Z2Nat.id, of_to_Z by assumption.
-      all: first [ reflexivity | lia ]. }
+    cbv [eqf Proper respectful]; revert A s; induction r; cbn [concretize]; intros A s t1 t2 H; auto; [].
+    destruct s.
+    eapply IHr; repeat intro; subst.
+    apply map_ext; intro.
+    apply H.
   Qed.
 
-  Definition reabstract {r : Rank} {A default s} (t_ : @tensor r A s) (t : @concrete_tensor r A s) : @tensor r A s
-    := let t := @abstract r A default s t in
-       fun idxs
-       => if (idxs <? s)%core
-          then t idxs
-          else t_ idxs.
+  #[export] Instance reabstract_Proper {r A default s} : Proper (eqf ==> eq ==> eqf) (@reabstract r A default s).
+  Proof. cbv [reabstract]; repeat intro; subst; match goal with |- context[match ?x with _ => _ end] => destruct x end; eauto. Qed.
 
-  Lemma reabstract_correct {r A default} {s : Shape r} {t_} {t} {idxs : RawIndex r}
-    : (forall
-          (in_bounds : is_true (match r with O => true | _ => idxs <? s end)%core),
-          abstract t idxs = t_ idxs)
-      -> @reabstract r A default s t_ t idxs = t_ idxs.
-  Proof.
-    cbv [reabstract].
-    repeat match goal with |- context[match ?x with _ => _ end] => destruct x eqn:? end.
-    all: auto.
-  Qed.
-
-  Lemma reabstract_ext_correct {r A default} {s : Shape r} {t_ t}
-    : t = @concretize r A s t_ -> forall idxs, @reabstract r A default s t_ t idxs = t_ idxs.
-  Proof. intros; subst; apply reabstract_correct, abstract_concretize. Qed.
-
-  Definition checkpoint {r : Rank} {A default s} t : @tensor r A s
-    := let t_ := t in
-       let t := @concretize r A s t in
-       @reabstract r A default s t_ t.
-
-  Lemma checkpoint_correct {r A default} {s : Shape r} {t} {idxs : RawIndex r}
-    : @checkpoint r A default s t idxs = t idxs.
-  Proof. cbv [checkpoint]; apply reabstract_ext_correct; reflexivity. Qed.
+  #[export] Instance checkpoint_Proper {r A default s} : Proper (eqf ==> eqf) (@checkpoint r A default s).
+  Proof. cbv [checkpoint]; repeat intro; subst; apply reabstract_Proper; try apply concretize_Proper; auto. Qed.
 End List.
+Export (hints) List.
 
-Definition adjust_index_for (s : ShapeType) : Index.IndexType -> RawIndex.IndexType
-  := fun i => i mod s.
-
-Definition adjust_indices_for {r} (s : Shape r) : Index r -> RawIndex r
-  := Index.map2 adjust_index_for s.
-
-Definition with_shape {r A} (s : Shape r) : @Shape.curriedT r A -> A
-  := fun f => Shape.uncurry f s.
-
-Notation of_array ls := (PArray.to_tensor ls) (only parsing).
-Notation of_list ls := (List.to_tensor ls) (only parsing).
-
-Definition repeat' {r A} (x : A) {s : Shape r} : tensor A s
-  := fun _ => x.
-Definition ones {r} {A} {one : has_one A} (s : Shape r) : tensor A s
-  := repeat' one.
-Definition zeros {r} {A} {zero : has_zero A} (s : Shape r) : tensor A s
-  := repeat' zero.
-
-Definition raw_get {r A} {s : Shape r} (t : tensor A s) (idxs : RawIndex r) : A
-  := t idxs.
-Definition get {r A} {s : Shape r} (t : tensor A s) (idxs : Index r) : A
-  := raw_get t (adjust_indices_for s idxs).
-Definition item {A} (t : tensor A []) : A := raw_get t tt.
-
-Notation "x .[ y ]" := (get x y) : tensor_scope.
-Notation "x .[ y ]" := (raw_get x y) : raw_tensor_scope.
-
+#[export] Instance raw_get_Proper {r A s} : Proper (eqf ==> eq ==> eq) (@raw_get r A s).
+Proof. cbv -[tensor RawIndex]; intros; subst; eauto. Qed.
+#[export] Instance get_Proper {r A s} : Proper (eqf ==> eq ==> eq) (@get r A s).
+Proof. cbv -[tensor RawIndex adjust_indices_for]; intros; subst; eauto. Qed.
+#[export] Instance item_Proper {A} : Proper (eqf ==> eq) (@item A) := _.
+(*
 Definition curried_raw_get {r A} {s : Shape r} (t : tensor A s) : @RawIndex.curriedT r A
   := RawIndex.curry (fun idxs => raw_get t idxs).
 Definition curried_get {r A} {s : Shape r} (t : tensor A s) : @Index.curriedT r A
   := Index.curry (fun idxs => get t idxs).
-
-Definition map {r A B} {s : Shape r} (f : A -> B) (t : tensor A s) : tensor B s
-  := fun i => f (t i).
-Definition map2 {r A B C} {sA sB : Shape r} (f : A -> B -> C) (tA : tensor A sA) (tB : tensor B sB) : tensor C (Shape.broadcast2 sA sB)
-  := fun i => f (tA i) (tB i).
-Definition map3 {r A B C D} {sA sB sC : Shape r} (f : A -> B -> C -> D) (tA : tensor A sA) (tB : tensor B sB) (tC : tensor C sC) : tensor D (Shape.broadcast3 sA sB sC)
-  := fun i => f (tA i) (tB i) (tC i).
-
-Definition map_dep {r A B} {s : Shape r} (f : forall a : A, B a) (t : tensor A s) : tensor_dep B t
-  := fun i => f (t i).
-
-
-Definition where_ {r A} {sA : Shape r} {sB : Shape r} {sC : Shape r} (condition : tensor bool sA) (input : tensor A sB) (other : tensor A sC) : tensor A (Shape.broadcast3 sA sB sC)
-  := map3 Bool.where_ condition input other.
-
-(* TODO: autobroadcast initial *)
-#[export] Instance tensor_add {r} {sA sB : Shape r} {A B C} {addA : has_add_with A B C} : has_add_with (tensor A sA) (tensor B sB) (tensor C (Shape.broadcast2 sA sB)) := map2 add.
-#[export] Instance tensor_sub {r} {sA sB : Shape r} {A B C} {subA : has_sub_with A B C} : has_sub_with (tensor A sA) (tensor B sB) (tensor C (Shape.broadcast2 sA sB)) := map2 sub.
-#[export] Instance tensor_mul {r} {sA sB : Shape r} {A B C} {mulA : has_mul_with A B C} : has_mul_with (tensor A sA) (tensor B sB) (tensor C (Shape.broadcast2 sA sB)) := map2 mul.
-#[export] Instance tensor_div_by {r} {sA sB : Shape r} {A B C} {div_byAB : has_div_by A B C} : has_div_by (tensor A sA) (tensor B sB) (tensor C (Shape.broadcast2 sA sB)) := map2 div.
-#[export] Instance tensor_sqrt {r} {s : Shape r} {A} {sqrtA : has_sqrt A} : has_sqrt (tensor A s) := map sqrt.
-#[export] Instance tensor_opp {r} {s : Shape r} {A} {oppA : has_opp A} : has_opp (tensor A s) := map opp.
-#[export] Instance add'1 {r} {s : Shape r} {a b} {A B C} {addA : has_add_with A B C} : has_add_with (tensor A (s ::' a)) (tensor B (s ::' b)) (tensor C (s ::' max a b)) | 10 := tensor_add.
-#[export] Instance sub'1 {r} {s : Shape r} {a b} {A B C} {subA : has_sub_with A B C} : has_sub_with (tensor A (s ::' a)) (tensor B (s ::' b)) (tensor C (s ::' max a b)) | 10 := tensor_sub.
-#[export] Instance mul'1 {r} {s : Shape r} {a b} {A B C} {mulA : has_mul_with A B C} : has_mul_with (tensor A (s ::' a)) (tensor B (s ::' b)) (tensor C (s ::' max a b)) | 10 := tensor_mul.
-#[export] Instance div_by'1 {r} {s : Shape r} {a b} {A B C} {div_byA : has_div_by A B C} : has_div_by (tensor A (s ::' a)) (tensor B (s ::' b)) (tensor C (s ::' max a b)) | 10 := tensor_div_by.
-#[export] Instance add'1s_r {r} {s : Shape r} {A B C} {addA : has_add_with A B C} : has_add_with (tensor A s) (tensor B (@Shape.ones r)) (tensor C s) | 10 := tensor_add.
-#[export] Instance add'1s_l {r} {s : Shape r} {A B C} {addA : has_add_with A B C} : has_add_with (tensor A (@Shape.ones r)) (tensor B s) (tensor C s) | 10 := tensor_add.
-#[export] Instance sub'1s_r {r} {s : Shape r} {A B C} {subA : has_sub_with A B C} : has_sub_with (tensor A s) (tensor B (@Shape.ones r)) (tensor C s) | 10 := tensor_sub.
-#[export] Instance sub'1s_l {r} {s : Shape r} {A B C} {subA : has_sub_with A B C} : has_sub_with (tensor A (@Shape.ones r)) (tensor B s) (tensor C s) | 10 := tensor_sub.
-#[export] Instance mul'1s_r {r} {s : Shape r} {A B C} {mulA : has_mul_with A B C} : has_mul_with (tensor A s) (tensor B (@Shape.ones r)) (tensor C s) | 10 := tensor_mul.
-#[export] Instance mul'1s_l {r} {s : Shape r} {A B C} {mulA : has_mul_with A B C} : has_mul_with (tensor A (@Shape.ones r)) (tensor B s) (tensor C s) | 10 := tensor_mul.
-#[export] Instance div_by'1s_r {r} {s : Shape r} {A B C} {div_byA : has_div_by A B C} : has_div_by (tensor A s) (tensor B (@Shape.ones r)) (tensor C s) | 10 := tensor_div_by.
-#[export] Instance div_by'1s_l {r} {s : Shape r} {A B C} {div_byA : has_div_by A B C} : has_div_by (tensor A (@Shape.ones r)) (tensor B s) (tensor C s) | 10 := tensor_div_by.
-#[export] Instance add'1s_r'1_same {r} {s : Shape r} {a} {A B C} {addA : has_add_with A B C} : has_add_with (tensor A (s ::' a)) (tensor B (@Shape.ones r ::' a)) (tensor C (s ::' a)) | 10 := tensor_add.
-#[export] Instance add'1s_l'1_same {r} {s : Shape r} {a} {A B C} {addA : has_add_with A B C} : has_add_with (tensor A (@Shape.ones r ::' a)) (tensor B (s ::' a)) (tensor C (s ::' a)) | 10 := tensor_add.
-#[export] Instance sub'1s_r'1_same {r} {s : Shape r} {a} {A B C} {subA : has_sub_with A B C} : has_sub_with (tensor A (s ::' a)) (tensor B (@Shape.ones r ::' a)) (tensor C (s ::' a)) | 10 := tensor_sub.
-#[export] Instance sub'1s_l'1_same {r} {s : Shape r} {a} {A B C} {subA : has_sub_with A B C} : has_sub_with (tensor A (@Shape.ones r ::' a)) (tensor B (s ::' a)) (tensor C (s ::' a)) | 10 := tensor_sub.
-#[export] Instance mul'1s_r'1_same {r} {s : Shape r} {a} {A B C} {mulA : has_mul_with A B C} : has_mul_with (tensor A (s ::' a)) (tensor B (@Shape.ones r ::' a)) (tensor C (s ::' a)) | 10 := tensor_mul.
-#[export] Instance mul'1s_l'1_same {r} {s : Shape r} {a} {A B C} {mulA : has_mul_with A B C} : has_mul_with (tensor A (@Shape.ones r ::' a)) (tensor B (s ::' a)) (tensor C (s ::' a)) | 10 := tensor_mul.
-#[export] Instance div_by'1s_r'1_same {r} {s : Shape r} {a} {A B C} {div_byA : has_div_by A B C} : has_div_by (tensor A (s ::' a)) (tensor B (@Shape.ones r ::' a)) (tensor C (s ::' a)) | 10 := tensor_div_by.
-#[export] Instance div_by'1s_l'1_same {r} {s : Shape r} {a} {A B C} {div_byA : has_div_by A B C} : has_div_by (tensor A (@Shape.ones r ::' a)) (tensor B (s ::' a)) (tensor C (s ::' a)) | 10 := tensor_div_by.
-#[export] Instance add'1s_r'1_same_app {r r'} {s : Shape r} {s' : Shape r'} {A B C} {addA : has_add_with A B C} : has_add_with (tensor A (s ++' s')) (tensor B (@Shape.ones r ++' s')) (tensor C (s ++' s')) | 10 := tensor_add.
-#[export] Instance add'1s_l'1_same_app {r r'} {s : Shape r} {s' : Shape r'} {A B C} {addA : has_add_with A B C} : has_add_with (tensor A (@Shape.ones r ++' s')) (tensor B (s ++' s')) (tensor C (s ++' s')) | 10 := tensor_add.
-#[export] Instance sub'1s_r'1_same_app {r r'} {s : Shape r} {s' : Shape r'} {A B C} {subA : has_sub_with A B C} : has_sub_with (tensor A (s ++' s')) (tensor B (@Shape.ones r ++' s')) (tensor C (s ++' s')) | 10 := tensor_sub.
-#[export] Instance sub'1s_l'1_same_app {r r'} {s : Shape r} {s' : Shape r'} {A B C} {subA : has_sub_with A B C} : has_sub_with (tensor A (@Shape.ones r ++' s')) (tensor B (s ++' s')) (tensor C (s ++' s')) | 10 := tensor_sub.
-#[export] Instance mul'1s_r'1_same_app {r r'} {s : Shape r} {s' : Shape r'} {A B C} {mulA : has_mul_with A B C} : has_mul_with (tensor A (s ++' s')) (tensor B (@Shape.ones r ++' s')) (tensor C (s ++' s')) | 10 := tensor_mul.
-#[export] Instance mul'1s_l'1_same_app {r r'} {s : Shape r} {s' : Shape r'} {A B C} {mulA : has_mul_with A B C} : has_mul_with (tensor A (@Shape.ones r ++' s')) (tensor B (s ++' s')) (tensor C (s ++' s')) | 10 := tensor_mul.
-#[export] Instance div_by'1s_r'1_same_app {r r'} {s : Shape r} {s' : Shape r'} {A B C} {div_byA : has_div_by A B C} : has_div_by (tensor A (s ++' s')) (tensor B (@Shape.ones r ++' s')) (tensor C (s ++' s')) | 10 := tensor_div_by.
-#[export] Instance div_by'1s_l'1_same_app {r r'} {s : Shape r} {s' : Shape r'} {A B C} {div_byA : has_div_by A B C} : has_div_by (tensor A (@Shape.ones r ++' s')) (tensor B (s ++' s')) (tensor C (s ++' s')) | 10 := tensor_div_by.
-
-(*
-Fixpoint extend_app_nil_l {P : Size -> Type} {s : Size} : P s -> P ([] ++' s)
-  := match s with
-     | [] => fun x => x
-     | s ::' _ => @extend_app_nil_l (fun s => P (s ::' _)) s
-     end.
-Fixpoint contract_app_nil_l {P : Size -> Type} {s : Size} : P ([] ++' s) -> P s
-  := match s with
-     | [] => fun x => x
-     | s ::' _ => @contract_app_nil_l (fun s => P (s ::' _)) s
-     end.
  *)
 
-Definition reshape_app_split' {A r1 r2 s1 s2} : @tensor (r1 +' r2) A (s1 ++' s2) -> tensor (tensor A s2) s1
-  := RawIndex.curry_radd.
-Definition reshape_app_combine' {A r1 r2 s1 s2} : tensor (tensor A s2) s1 -> @tensor (r1 +' r2) A (s1 ++' s2)
-  := RawIndex.uncurry_radd.
-(* infer s1 s2 from the conclusion *)
-#[global] Arguments reshape_app_combine' A & r1 r2 s1 s2 _.
-#[global] Arguments reshape_app_split' A & r1 r2 s1 s2 _.
-Definition reshape_app_split {A r1 r2 s1 s2} : @tensor (r1 +' r2) A (s1 ++' s2) -> tensor (tensor A s2) s1
-  := reshape_app_split'.
-Definition reshape_app_combine {A r1 r2 s1 s2} : tensor (tensor A s2) s1 -> @tensor (r1 +' r2) A (s1 ++' s2)
-  := reshape_app_combine'.
-Definition reshape_snoc_split {A r s1 s2} : @tensor (r +' 1) A (s1 ::' s2) -> tensor (tensor A [s2]) s1
-  := RawIndex.curry_radd.
-Definition reshape_snoc_combine {A r s1 s2} : tensor (tensor A [s2]) s1 -> @tensor (r +' 1) A (s1 ::' s2)
-  := RawIndex.uncurry_radd.
+Local Ltac t_step :=
+  first [ progress subst
+        | intro
+        | reflexivity
+        | match goal with
+          | [ H : context[_ = _] |- _ ] => rewrite H
+          end
+        | solve [ eauto ]
+        | match goal with
+          | [ |- context[match ?x with _ => _ end] ] => destruct x eqn:?
+          end ].
+Local Ltac t := repeat t_step.
+
+#[export] Instance map_Proper_R {r A B s RA RB} : Proper ((RA ==> RB) ==> eqfR RA ==> eqfR RB) (@map r A B s).
+Proof. cbv -[tensor RawIndex]; t. Qed.
+#[export] Instance map2_Proper_R {r A B C sA sB RA RB RC} : Proper ((RA ==> RB ==> RC) ==> eqfR RA ==> eqfR RB ==> eqfR RC) (@map2 r A B C sA sB).
+Proof. cbv -[tensor RawIndex]; t. Qed.
+#[export] Instance map3_Proper_R {r A B C D sA sB sC RA RB RC RD} : Proper ((RA ==> RB ==> RC ==> RD) ==> eqfR RA ==> eqfR RB ==> eqfR RC ==> eqfR RD) (@map3 r A B C D sA sB sC).
+Proof. cbv -[tensor RawIndex]; t. Qed.
+
+#[export] Instance map_Proper {r A B s RB} : Proper (pointwise_relation _ RB ==> eqf ==> eqfR RB) (@map r A B s).
+Proof. repeat intro; eapply map_Proper_R; try eassumption; repeat intro; subst; eauto. Qed.
+#[export] Instance map2_Proper {r A B C sA sB R} : Proper (pointwise_relation _ (pointwise_relation _ R) ==> eqf ==> eqf ==> eqfR R) (@map2 r A B C sA sB).
+Proof. repeat intro; eapply map2_Proper_R; try eassumption; repeat intro; subst; cbv [pointwise_relation] in *; eauto. Qed.
+#[export] Instance map3_Proper {r A B C D sA sB sC R} : Proper (pointwise_relation _ (pointwise_relation _ (pointwise_relation _ R)) ==> eqf ==> eqf ==> eqf ==> eqfR R) (@map3 r A B C D sA sB sC).
+Proof. repeat intro; eapply map3_Proper_R; try eassumption; repeat intro; subst; cbv [pointwise_relation] in *; eauto. Qed.
+(*
+Definition map_dep {r A B} {s : Shape r} (f : forall a : A, B a) (t : tensor A s) : tensor_dep B t
+  := fun i => f (t i).
+*)
+#[export] Instance where__Proper {r A sA sB sC} : Proper (eqf ==> eqf ==> eqf ==> eqf) (@where_ r A sA sB sC).
+Proof. apply map3_Proper; repeat intro; reflexivity. Qed.
+
+#[export] Instance tensor_add_Proper {r sA sB A B C addA RA RB RC} {_ : Proper (RA ==> RB ==> RC) addA} : Proper (eqfR RA ==> eqfR RB ==> eqfR RC) (@tensor_add r sA sB A B C addA).
+Proof. cbv [tensor_add add]; repeat intro; eapply map2_Proper_R; eassumption. Qed.
+#[export] Instance tensor_sub_Proper {r sA sB A B C subA RA RB RC} {_ : Proper (RA ==> RB ==> RC) subA} : Proper (eqfR RA ==> eqfR RB ==> eqfR RC) (@tensor_sub r sA sB A B C subA).
+Proof. cbv [tensor_sub sub]; repeat intro; eapply map2_Proper_R; eassumption. Qed.
+#[export] Instance tensor_mul_Proper {r sA sB A B C mulA RA RB RC} {_ : Proper (RA ==> RB ==> RC) mulA} : Proper (eqfR RA ==> eqfR RB ==> eqfR RC) (@tensor_mul r sA sB A B C mulA).
+Proof. cbv [tensor_mul mul]; repeat intro; eapply map2_Proper_R; eassumption. Qed.
+#[export] Instance tensor_div_by_Proper {r sA sB A B C div_byA RA RB RC} {_ : Proper (RA ==> RB ==> RC) div_byA} : Proper (eqfR RA ==> eqfR RB ==> eqfR RC) (@tensor_div_by r sA sB A B C div_byA).
+Proof. cbv [tensor_div_by div]; repeat intro; eapply map2_Proper_R; eassumption. Qed.
+#[export] Instance tensor_sqrt_Proper {r s A sqrtA R} {_ : Proper (R ==> R) sqrtA} : Proper (eqfR R ==> eqfR R) (@tensor_sqrt r s A sqrtA).
+Proof. cbv [tensor_sqrt sqrt]; repeat intro; eapply map_Proper_R; eassumption. Qed.
+#[export] Instance tensor_opp_Proper {r s A oppA R} {_ : Proper (R ==> R) oppA} : Proper (eqfR R ==> eqfR R) (@tensor_opp r s A oppA).
+Proof. cbv [tensor_opp opp]; repeat intro; eapply map_Proper_R; eassumption. Qed.
+
+
+#[export] Instance reshape_app_split'_Proper {A r1 r2 s1 s2 R} : Proper (eqfR R ==> eqfR (eqfR R)) (@reshape_app_split' A r1 r2 s1 s2).
+Proof.
+  cbv [reshape_app_split' RawIndex.curry_radd].
+  repeat intro; eauto.
+Qed.
+#[export] Instance reshape_app_combine'_Proper {A r1 r2 s1 s2 R} : Proper (eqfR (eqfR R) ==> eqfR R) (@reshape_app_combine' A r1 r2 s1 s2).
+Proof.
+  cbv [reshape_app_combine' RawIndex.uncurry_radd].
+  repeat intro; destruct RawIndex.split_radd; cbv [eqfR pointwise_relation] in *; eauto.
+Qed.
+#[export] Instance reshape_app_split_Proper {A r1 r2 s1 s2 R} : Proper (eqfR R ==> eqfR (eqfR R)) (@reshape_app_split A r1 r2 s1 s2) := _.
+#[export] Instance reshape_app_combine_Proper {A r1 r2 s1 s2 R} : Proper (eqfR (eqfR R) ==> eqfR R) (@reshape_app_combine A r1 r2 s1 s2) := _.
+#[export] Instance reshape_snoc_split_Proper {A r s1 s2 R} : Proper (eqfR R ==> eqfR (eqfR R)) (@reshape_snoc_split A r s1 s2).
+Proof.
+  cbv [reshape_snoc_split RawIndex.curry_radd].
+  repeat intro; eauto.
+Qed.
+#[export] Instance reshape_snoc_combine_Proper {A r s1 s2 R} : Proper (eqfR (eqfR R) ==> eqfR R) (@reshape_snoc_combine A r s1 s2).
+Proof.
+  cbv [reshape_snoc_combine RawIndex.uncurry_radd].
+  repeat intro; destruct RawIndex.split_radd; cbv [eqfR pointwise_relation] in *; eauto.
+Qed.
+(*
 Definition uncurry {r A} {s : Shape r} : @RawIndex.curriedT r A -> tensor A s
   := RawIndex.uncurry.
 Definition curry {r A} {s : Shape r} : tensor A s -> @RawIndex.curriedT r A
   := RawIndex.curry.
-
-Definition map' {ra1 ra2 rb A B} {sa1 : Shape ra1} {sa2 : Shape ra2} {sb : Shape rb} (f : tensor A sa2 -> tensor B sb) (t : tensor A (sa1 ++' sa2)) : tensor B (sa1 ++' sb)
-  := reshape_app_combine (map f (reshape_app_split t)).
-Definition map2' {ri1 ri2 ro A B C} {sA1 sB1 : Shape ri1} {sA2 sB2 : Shape ri2} {so : Shape ro} (f : tensor A sA2 -> tensor B sB2 -> tensor C so) (tA : tensor A (sA1 ++' sA2)) (tB : tensor B (sB1 ++' sB2)) : tensor C (Shape.broadcast2 sA1 sB1 ++' so)
-  := reshape_app_combine (map2 f (reshape_app_split tA) (reshape_app_split tB)).
-
-(*
-Definition reshape_S_fun_combine {I A} {r : Rank} : (I -> tensor_fun_of_rank I A r) -> tensor_fun_of_rank I A (1 +' r)
-  := match reshape_app_combine_gen (r1:=1) (r2:=r) with x => x end.
-Definition reshape_S_fun_split {I A} {r : Rank} : tensor_fun_of_rank I A (1 +' r) -> (I -> tensor_fun_of_rank I A r)
-  := match reshape_app_split_gen (r1:=1) (r2:=r) with x => x end.
-*)
-(*
-Require Import Program . Obligation Tactic := cbn; intros.
-Fixpoint broadcast_map_ {A B} {s1 s2 : Size} {keepdim : with_default bool false} (f : A -> tensor_of_shape B s2) {struct s1} : tensor_of_shape A s1 -> tensor_of_shape (tensor_of_shape B (s1 ++' (if keepdim then [1] else []) ++' s2) s1.
-refine match s1, keepdim return tensor_of_shape A s1 -> tensor_of_shape B (s1 ++' (if keepdim then [1] else []) ++' s2) with
-     | [], true => fun x => reshape_app_combine (s1:=[1]) (PArray.make 1 (f x))
-     | [], false => fun x => reshape_app_combine (s1:=[]) (f x)
-     | s1 ::' _, keepdim
-       => fun x => _ (*(broadcast_map (keepdim:=keepdim) (s1:=s1)) (* _(*PArray.map f*))*)*)
-       end; cbn in *.
-epose (@broadcast_map _ _ s1 _ keepdim _ x).
-epose (@broadcast_map _ _ s1 _ keepdim (fun a => reshape_app_combine (s1:=[1])).
-Next Obligation.
-  pose (
- pose (broa
-
-Fixpoint extended_broadcast_map {A B} {s1 s1' s2 : Size} (f : tensor_of_shape A s1' -> tensor_of_shape B s2) {struct s1} : tensor_of_shape A (s1 ++ s1') -> tensor_of_shape B (s1 ++ s2)
-  := match s1 with
-     | [] => f
-     | s :: s1
-       => PArray.map (extended_broadcast_map f)
-     end.
- *)
-
-(*
-Definition broadcast_m1 {A s} n : tensor_of_shape A s -> tensor_of_shape A (s ::' n)
-  := tensor_map (PArray.make n).
-Definition broadcast_0 {A s} n : tensor_of_shape A s -> tensor_of_shape A ([n] ++' s)
-  := fun x => reshape_app_combine (PArray.make n x).
-#[global] Arguments broadcast_m1 A & s n _.
-#[global] Arguments broadcast_0 A & s n _.
-Definition slice_none_m1 {A s} : tensor_of_shape A s -> tensor_of_shape A (s ::' 1)
-  := broadcast_m1 1.
-Definition slice_none_0 {A s} : tensor_of_shape A s -> tensor_of_shape A ([1] ++' s)
-  := broadcast_0 1.
 *)
 
-Definition broadcast' {A} (x : A) {r : Rank} : tensor A (@Shape.ones r)
-  := repeat' x.
-Definition broadcast {r A} {s : Shape r} (x : tensor A s) {r' : Rank} : tensor A (@Shape.ones r' ++' s)
-  := reshape_app_combine (broadcast' x).
-Definition repeat {r A} {s : Shape r} (x : tensor A s) {r' : Rank} (s' : Shape r') : tensor A (s' ++' s)
-  := reshape_app_combine (repeat' x (s:=s')).
+#[export] Instance map'_Proper {ra1 ra2 rb A B sa1 sa2 sb RA RB} : Proper ((eqfR RA ==> eqfR RB) ==> eqfR RA ==> eqfR RB) (@map' ra1 ra2 rb A B sa1 sa2 sb).
+Proof.
+  cbv [map']; repeat intro.
+  apply reshape_app_combine_Proper.
+  eapply map_Proper_R; try eassumption.
+  apply reshape_app_split_Proper; eassumption.
+Qed.
+#[export] Instance map2'_Proper {ri1 ri2 ro A B C sA1 sB1 sA2 sB2 so RA RB RC} : Proper ((eqfR RA ==> eqfR RB ==> eqfR RC) ==> eqfR RA ==> eqfR RB ==> eqfR RC) (@map2' ri1 ri2 ro A B C sA1 sB1 sA2 sB2 so).
+Proof.
+  cbv [map2']; repeat intro.
+  apply reshape_app_combine_Proper.
+  eapply map2_Proper_R; try eassumption.
+  all: apply reshape_app_split_Proper; eassumption.
+Qed.
 
-Definition keepdim_gen {r} {s : Shape r} {A B} (f : A -> tensor B s) : A -> tensor B ([1] ++' s)
-  := fun a => broadcast (f a).
-Definition keepdim {A B} (f : A -> B) : A -> tensor B [1] := keepdim_gen (s:=[]) (fun a 'tt => f a).
-#[local] Notation keepdimf := keepdim (only parsing).
+#[export] Instance broadcast_Proper {r A s R} : Proper (eqfR R ==> forall_relation (fun r' => eqfR R)) (@broadcast r A s).
+Proof.
+  cbv [broadcast broadcast' repeat']; intros ??? ?.
+  apply reshape_app_combine_Proper.
+  intro; assumption.
+Qed.
+#[export] Instance repeat_Proper {r A s R} : Proper (eqfR R ==> forall_relation (fun r' => forall_relation (fun s' => eqfR R))) (@repeat r A s).
+Proof.
+  cbv [repeat repeat']; intros ??? ? ?.
+  apply reshape_app_combine_Proper.
+  intro; assumption.
+Qed.
 
-Definition reduce_axis_m1' {r A B} {s1 : Shape r} {s2}
-  (reduction : forall (start stop step : RawIndexType), (RawIndexType -> A) -> B)
-  (t : tensor A (s1 ::' s2))
-  : tensor B s1
-  := map (fun v => reduction 0 s2 1 (fun i => raw_get v [i])) (reshape_snoc_split t).
+#[export] Instance keepdim_gen_Proper {r s A B R} : Proper (pointwise_relation _ (eqfR R) ==> eq ==> eqfR R) (@keepdim_gen r s A B).
+Proof.
+  cbv [keepdim_gen]; intros ?? H ???; subst.
+  apply broadcast_Proper; apply H.
+Qed.
+#[export] Instance keepdim_Proper {A B R} : Proper (pointwise_relation _ R ==> eq ==> eqfR R) (@keepdim A B).
+Proof.
+  cbv [keepdim]; intros ?? H ??? ?; subst; eapply keepdim_gen_Proper; t.
+Qed.
 
-Definition reduce_axis_m1 {r A B} {s1 : Shape r} {s2} {keepdim : with_default "keepdim" bool false}
-  (reduction : forall (start stop step : RawIndexType), (RawIndexType -> A) -> B)
-  : tensor A (s1 ::' s2) -> tensor B (s1 ++' if keepdim return Shape (if keepdim then _ else _) then [1] else [])
-  := if keepdim
-          return tensor A (s1 ::' s2) -> tensor B (s1 ++' if keepdim return Shape (if keepdim then _ else _) then [1] else [])
-     then fun t idxs => reduce_axis_m1' reduction t (RawIndex.hd idxs)
-     else reduce_axis_m1' reduction.
+#[export] Instance reduce_axis_m1'_Proper {r A B s1 s2 RA RB} : Proper (pointwise_relation _ (pointwise_relation _ (pointwise_relation _ (pointwise_relation _ RA ==> RB))) ==> eqfR RA ==> eqfR RB) (@reduce_axis_m1' r A B s1 s2).
+Proof.
+  cbv [reduce_axis_m1'].
+  intros ?? H ?? Ht.
+  eapply map_Proper_R; try eapply reshape_snoc_split_Proper; try eassumption.
+  intros ?? Ht'.
+  cbv [pointwise_relation eqfR respectful] in *.
+  eauto.
+Qed.
 
-Definition softmax_dim_m1 {r A B C} {addB : has_add B} {expA : has_exp_to A B} {zeroB : has_zero B} {divB : has_div_by B B C} {s0 : Shape r} {s'} (s:=(s0 ::' s')%shape) (t : tensor A s) : tensor C s
-  := (let exp_t : tensor B s := map exp t in
-      let sum_exp_t : tensor B s := reduce_axis_m1 (keepdim:=true) sum exp_t in
-      exp_t / sum_exp_t)%core.
+#[export] Instance reduce_axis_m1_Proper {r A B s1 s2 keepdim RA RB}
+  : Proper (pointwise_relation _ (pointwise_relation _ (pointwise_relation _ (pointwise_relation _ RA ==> RB))) ==> eqfR RA ==> eqfR RB)
+      (@reduce_axis_m1 r A B s1 s2 keepdim).
+Proof.
+  cbv [reduce_axis_m1]; destruct keepdim; intros ?? H ?? Ht ?.
+  all: eapply reduce_axis_m1'_Proper; try eassumption.
+Qed.
 
-Definition log_softmax_dim_m1 {r A B C D} {addB : has_add B} {lnA : has_ln_to B C} {expA : has_exp_to A B} {zeroB : has_zero B} {divB : has_div_by A C D} {s0 : Shape r} {s'} (s:=(s0 ::' s')%shape) (t : tensor A s) : tensor D s
-  := (let exp_t : tensor B s := map exp t in
-      let sum_exp_t : tensor B s := reduce_axis_m1 (keepdim:=true) sum exp_t in
-      let ln_sum_exp_t : tensor C s := map ln sum_exp_t in
-      t / ln_sum_exp_t)%core.
 
-Definition unsqueeze_dim_m1 {A r} {s : Shape r} (t : tensor A s) : tensor A (s ::' 1)
-  := fun idxs => raw_get t (RawIndex.hd idxs).
+(*#[export] Instance reduce_axis_m1'_Proper' {r A B s1 s2 reduction RA} : Proper (eqfR RA ==> eqf) (@reduce_axis_m1' r A B s1 s2 reduction).
+Proof.
+  cbv [reduce_axis_m1'].
+  intros ?? Ht.
+  eapply map_Proper_R; try eapply reshape_snoc_split_Proper; try eassumption.
+  intros ?? Ht'.
+  cbv [pointwise_relation eqfR respectful] in *.
+  eauto.
+Qed.
 
-Definition gather_dim_m1 {A r} {ssinput ssindex : Shape r} {sinput' sindex'}
-  (sinput := (ssinput ::' sinput')%shape) (sindex := (ssindex ::' sindex')%shape)
-  (input : tensor A sinput)
-  (index : tensor IndexType sindex)
-  : tensor A sindex
-  := fun idx => raw_get input (RawIndex.hd idx ::' adjust_index_for sinput' (raw_get index idx))%raw_index.
+#[export] Instance reduce_axis_m1_Proper {r A B s1 s2 keepdim RA RB}
+  : Proper (pointwise_relation _ (pointwise_relation _ (pointwise_relation _ (pointwise_relation _ RA ==> RB))) ==> eqfR RA ==> eqfR RB)
+      (@reduce_axis_m1 r A B s1 s2 keepdim).
+Proof.
+  cbv [reduce_axis_m1]; destruct keepdim; intros ?? H ?? Ht ?.
+  all: eapply reduce_axis_m1'_Proper; try eassumption.
+Qed.
 
-Definition squeeze {r A} {s : Shape r} (t : tensor A s) : tensor A (Shape.squeeze s)
-  := fun idx => raw_get t (RawIndex.unsqueeze idx).
-
-Definition reshape_m1 {A r} {s : Shape r} (t : tensor A s) : tensor A (Shape.reshape s)
-  := fun idx => raw_get t (RawIndex.unreshape s idx).
-Definition unreshape_m1 {A r} {s : Shape r} (t : tensor A (Shape.reshape s)) : tensor A s
-  := fun idx => raw_get t (RawIndex.reshape s idx).
-(*
-Definition reshape {A r1 r2} {s1 : Shape r1} (t : tensor A s1) (s2 : Shape r2) : tensor A s2
-  := unreshape_m1 (reshape_m1 t : tensor A (Shape.reshape s2)).
- *)
-
-Definition to_bool {A} {zero : has_zero A} {eqb : has_eqb A} {r} {s : Shape r} (xs : tensor A s) : tensor bool s
-  := map (fun x => x ≠? 0)%core xs.
-
-Definition of_bool {A} {zero : has_zero A} {one : has_one A} {r} {s : Shape r} (xs : tensor bool s) : tensor A s
-  := map (fun x:bool => if x then 1 else 0)%core xs.
-
-Definition mean {r A} {s : Shape r} {B C} {zero : has_zero A} {add : has_add A} {div_by : has_div_by A B C} {coer : has_coer Z B} (t : tensor A s) : tensor C []
-  := reduce_axis_m1 Reduction.mean (reshape_m1 t).
-(*
-Definition arange {A B} {START STOP STEP IDX} {oneA : has_one A} {zeroStart : has_zero START} {oneStep : has_one STEP} {sub : has_sub_with STOP START A} {subA : has_sub A} {div : has_int_div_by A STEP B} {coerZ : has_coer B Z} {coerIDX : has_coer int IDX} {add : has_add_with START C D} {mul : has_mul_with STEP IDX C}
-  {start : with_default "start" START 0%core} (stop : STOP) {step : with_default "step" STEP 1%core}
-  : tensor int [(1 + Uint63.of_Z (((stop - start) - 1) // step))%core%uint63]
-  := fun idx => let idx := RawIndex.item idx in
-                (start + idx * step)%uint63.
 *)
-Definition arange {start : with_default "start" int 0%uint63} (stop : int) {step : with_default "step" int 1%uint63}
-  : tensor int [(1 + (stop - start - 1) / step)%uint63]
-  := fun idx => let idx := RawIndex.item idx in
-                (start + idx * step)%uint63.
+#[export] Instance softmax_dim_m1_Proper {r A B C addB expA zeroB divB s0 s'}
+  : Proper (eqf ==> eqf) (@softmax_dim_m1 r A B C addB expA zeroB divB s0 s').
+Proof.
+  intros ?? Ht.
+  cbv [softmax_dim_m1 div].
+  eapply tensor_div_by_Proper.
+  all: try eapply (@reduce_axis_m1_Proper r B B s0 s' true).
+  all: try (eapply map_Proper; try eassumption; repeat intro).
+  all: try eapply sum_Proper_pointwise.
+  all: try exact eq_refl.
+  Unshelve.
+  repeat intro; subst; reflexivity.
+Qed.
 
-#[global] Arguments arange (_ _ _)%uint63.
-#[global] Arguments arange {_} _ {_}, _ _ {_}, _ _ _.
+#[export] Instance log_softmax_dim_m1_Proper {r A B C D addB lnA expA zeroB divB s0 s'}
+  : Proper (eqf ==> eqf) (@log_softmax_dim_m1 r A B C D addB lnA expA zeroB divB s0 s').
+Proof.
+  intros ?? Ht.
+  cbv [log_softmax_dim_m1 div].
+  eapply tensor_div_by_Proper; try eassumption.
+  eapply map_Proper; try eassumption.
+  all: try eapply (@reduce_axis_m1_Proper r B B s0 s' true).
+  all: try (eapply map_Proper; try eassumption; repeat intro).
+  all: try eapply sum_Proper_pointwise.
+  all: try (repeat intro; exact eq_refl).
+  Unshelve.
+  repeat intro; subst; reflexivity.
+Qed.
 
-(* TODO: nary *)
+#[export] Instance unsqueeze_dim_m1_Proper {A r s R} : Proper (eqfR R ==> eqfR R) (@unsqueeze_dim_m1 A r s).
+Proof. intros ?? H; cbv; intros; apply H. Qed.
+
+#[export] Instance gather_dim_m1_Proper {A r ssinput ssindex sinput' sindex' R} : Proper (eqfR R ==> eqf ==> eqfR R) (@gather_dim_m1 A r ssinput ssindex sinput' sindex').
+Proof.
+  intros ?? H1 ?? H2; cbv [gather_dim_m1]; intro.
+  rewrite H2.
+  apply H1.
+Qed.
+
+#[export] Instance squeeze_Proper {A r s R} : Proper (eqfR R ==> eqfR R) (@squeeze A r s).
+Proof. intros ?? H; cbv; intros; apply H. Qed.
+#[export] Instance reshape_m1_Proper {A r s R} : Proper (eqfR R ==> eqfR R) (@reshape_m1 A r s).
+Proof. intros ?? H ?; cbv [reshape_m1]; apply H. Qed.
+#[export] Instance unreshape_m1_Proper {A r s R} : Proper (eqfR R ==> eqfR R) (@unreshape_m1 A r s).
+Proof. intros ?? H ?; cbv [unreshape_m1]; apply H. Qed.
+
+#[export] Instance to_bool_Proper {A zero eqb r s} : Proper (eqf ==> eqf) (@to_bool A zero eqb r s).
+Proof.
+  intros ?? H ?; cbv [to_bool]; apply map_Proper; try assumption; repeat intro; reflexivity.
+Qed.
+
+#[export] Instance of_bool_Proper {A zero one r s} : Proper (eqf ==> eqf) (@of_bool A zero one r s).
+Proof.
+  intros ?? H ?; cbv [of_bool]; apply map_Proper; try assumption; repeat intro; reflexivity.
+Qed.
+
+
+#[export] Instance mean_Proper {r A s B C zero addA div_boyABC coerB} : Proper (eqf ==> eqf) (@mean r A s B C zero addA div_boyABC coerB).
+Proof.
+  cbv [mean]; intros ?? H ?.
+  eapply reduce_axis_m1_Proper.
+  1: eapply mean_Proper_pointwise.
+  apply reshape_m1_Proper.
+  assumption.
+Qed.
+
+(*(* TODO: nary *)
 Definition tupleify {A B s1 s2} (t1 : tensor A [s1]) (t2 : tensor B [s2]) : tensor (A * B) [s1; s2]
   := fun '((tt, a), b) => (raw_get t1 [a], raw_get t2 [b]).
 Definition cartesian_prod {A s1 s2} (t1 : tensor A [s1]) (t2 : tensor A [s2]) : tensor A [s1 * s2; 2]
   := fun '((tt, idx), tuple_idx)
      => let '(a, b) := raw_get (reshape_m1 (tupleify t1 t2)) [idx] in
         nth_default a [a; b] (Z.to_nat (Uint63.to_Z (tuple_idx mod 2))).
-
-(** Quoting https://pytorch.org/docs/stable/generated/torch.tril.html
-
-torch.tril(input, diagonal=0, *, out=None) → Tensor
-
-Returns the lower triangular part of the matrix (2-D tensor) or batch
-of matrices [input], the other elements of the result tensor [out] are
-set to 0.
-
-The lower triangular part of the matrix is defined as the elements on
-and below the diagonal.
-
-The argument [diagonal] controls which diagonal to consider. If
-[diagonal = 0], all elements on and below the main diagonal are
-retained. A positive value includes just as many diagonals above the
-main diagonal, and similarly a negative value excludes just as many
-diagonals below the main diagonal. The main diagonal are the set of
-indices {(i,i)} for i ∈ [0,min{d₁,d₂}−1] where d₁,d₂ are the
-dimensions of the matrix. *)
-Definition tril {A} {zero : has_zero A} {rnk} {s : Shape rnk} {r c}
-  {diagonal : with_default "diagonal" int 0%int63} (input : tensor A (s ++' [r; c]))
-  : tensor A (s ++' [r; c])
-  := fun '(((_, i), j) as idxs)
-     => if ((0 ≤? i) && (i <? r) && (Sint63.max 0 (1 + i + diagonal) ≤? j) && (j <? c))%bool
-        then 0%core
-        else input idxs.
-#[global] Arguments tril {A%type_scope zero rnk%nat s%shape} {r c}%uint63 {diagonal}%sint63 input%tensor.
-(** Quoting https://pytorch.org/docs/stable/generated/torch.triu.html
-
-torch.triu(input, diagonal=0, *, out=None) → Tensor
-
-Returns the upper triangular part of the matrix (2-D tensor) or batch
-of matrices [input], the other elements of the result tensor [out] are
-set to 0.
-
-The upper triangular part of the matrix is defined as the elements on
-and above the diagonal.
-
-The argument [diagonal] controls which diagonal to consider. If
-[diagonal = 0], all elements on and above the main diagonal are
-retained. A positive value excludes just as many diagonals above the
-main diagonal, and similarly a negative value includes just as many
-diagonals below the main diagonal. The main diagonal are the set of
-indices {(i,i)} for i ∈ [0,min{d₁,d₂}−1] where d₁,d₂ are the
-dimensions of the matrix. *)
-Definition triu {A} {zero : has_zero A} {rnk} {s : Shape rnk} {r c}
-  {diagonal : with_default "diagonal" int 0%int63} (input : tensor A (s ++' [r; c]))
-  : tensor A (s ++' [r; c])
-  := fun '(((_, i), j) as idxs)
-     => if ((0 ≤? i) && (i <? r) && (0 ≤? j) && (j <? Sint63.max 0 (i + diagonal)))%bool
-        then 0%core
-        else input idxs.
-#[global] Arguments triu {A%type_scope zero rnk%nat s%shape} {r c}%uint63 {diagonal}%sint63 input%tensor.
+ *)
+#[export] Instance tril_Proper {A zeroA rnk s r c diagonal} : Proper (eqf ==> eqf) (@tril A zeroA rnk s r c diagonal).
+Proof.
+  cbv [tril]; intros ?? H [[? ?] ?].
+  rewrite H.
+  reflexivity.
+Qed.
+#[export] Instance triu_Proper {A zeroA rnk s r c diagonal} : Proper (eqf ==> eqf) (@triu A zeroA rnk s r c diagonal).
+Proof.
+  cbv [triu]; intros ?? H [[? ?] ?].
+  rewrite H.
+  reflexivity.
+Qed.
